Impl/QueryModel.i.dfy
@@ -12,6 +12,9 @@ module QueryModel {
   import opened IOModel
   import opened BookkeepingModel
   import opened EvictModel
+  import opened KeyType
+  import ValueType
+  import opened ValueMessage
 
   import opened Options
   import opened Maps
@@ -29,7 +32,7 @@ module QueryModel {
   // == query ==
 
   predicate {:opaque} queryIterate(k: Constants, s: Variables, key: Key, msg: Message, ref: BT.G.Reference, io: IO, counter: uint64,
-      s': Variables, result: Option<MS.Value>, io': IO)    
+      s': Variables, result: Option<Value>, io': IO)    
   requires s.Ready?
   requires Inv(k, s)
   requires io.IOInit?
@@ -66,7 +69,7 @@ module QueryModel {
             queryIterate(k, s0, key, newmsg, node.children.value[r], io, counter - 1, s', result, io')
           ) else (
             && s' == s0
-            && result == Some(MS.V.DefaultValue())
+            && result == Some(ValueType.DefaultValue())
             && io' == io
           )
         )
@@ -74,8 +77,8 @@ module QueryModel {
     )
   }
 
-  predicate {:opaque} query(k: Constants, s: Variables, io: IO, key: MS.Key,
-      s': Variables, result: Option<MS.Value>, io': IO)
+  predicate {:opaque} query(k: Constants, s: Variables, io: IO, key: Key,
+      s': Variables, result: Option<Value>, io': IO)
   requires io.IOInit?
   requires Inv(k, s)
   {
@@ -105,7 +108,7 @@ module QueryModel {
     && msg == BT.InterpretLookup(lookup, key)
   }
 
-  lemma AugmentLookup(lookup: seq<BT.G.ReadOp>, ref: BT.G.Reference, node: BT.G.Node, key: MS.Key, cache: map<BT.G.Reference, BT.G.Node>, graph: map<BT.G.Reference, seq<BT.G.Reference>>)
+  lemma AugmentLookup(lookup: seq<BT.G.ReadOp>, ref: BT.G.Reference, node: BT.G.Node, key: Key, cache: map<BT.G.Reference, BT.G.Node>, graph: map<BT.G.Reference, seq<BT.G.Reference>>)
   returns (lookup' : seq<BT.G.ReadOp>)
   requires |lookup| > 0 ==> BT.WFLookupForKey(lookup, key)
   requires forall i | 0 <= i < |lookup| :: lookup[i].ref in graph
@@ -138,7 +141,7 @@ module QueryModel {
   }
 
   lemma queryIterateCorrect(k: Constants, s: Variables, key: Key, msg: Message, ref: BT.G.Reference, io: IO, counter: uint64, lookup: seq<BT.G.ReadOp>,
-      s': Variables, res: Option<MS.Value>, io': IO)
+      s': Variables, res: Option<Value>, io': IO)
   requires queryInv(k, s, key, msg, ref, io, counter, lookup)
   requires !msg.Define?
   requires queryIterate(k, s, key, msg, ref, io, counter, s', res, io');
@@ -208,8 +211,8 @@ module QueryModel {
     }
   }
 
-  lemma queryCorrect(k: Constants, s: Variables, io: IO, key: MS.Key,
-      s': Variables, res: Option<MS.Value>, io': IO)
+  lemma queryCorrect(k: Constants, s: Variables, io: IO, key: Key,
+      s': Variables, res: Option<Value>, io': IO)
   requires io.IOInit?
   requires Inv(k, s)
   requires query(k, s, io, key, s', res, io');
